src/lib/qasm2/api.mli
@@ -7,5 +7,5 @@ module Desugar = Desugar
 val parse_string : string -> Ast.program
 val get_ast : string -> Ast.program
 val inline_qelib : Ast.program -> Ast.program
-val desugar : Ast.program -> int * Extracted.inlinedProgram * Desugar.QASMArg.t Desugar.IntMap.t * Desugar.QASMArg.t Desugar.IntMap.t
+val desugar : Ast.program -> int * int * Extracted.instruction * Desugar.QASMArg.t Desugar.IntMap.t * Desugar.QASMArg.t Desugar.IntMap.t
 val string_of_instruction : Extracted.instruction -> string
